FMT/Types/LocalType.lean
@@ -1,5 +1,12 @@
 namespace FMT.Types
 
-abbrev LocalType : Type := Bool
+inductive LocalType : Type
+| zero
+| one
+deriving DecidableEq, Repr
+
+def evalLocal : LocalType → Nat
+| .zero => 0
+| .one  => 1
 
 end FMT.Types
